rustfrontend/RustIRcfg.v
@@ -28,17 +28,70 @@ Inductive select_kind : Type :=
 
 Definition selector := list select_kind.
 
-Fixpoint select_stmt (stmt: statement) (sel: selector) : option statement :=
+
+Definition select_stmt_aux (sel: select_kind) (stmt: option statement) : option statement :=
   match sel, stmt with
-  | nil, _ => Some stmt
-  | Selseqleft :: sel', Ssequence s1 s2 => select_stmt s1 sel'
-  | Selseqright :: sel', Ssequence s1 s2 => select_stmt s2 sel'
-  | Selifthen :: sel', Sifthenelse _ s1 s2 => select_stmt s1 sel'
-  | Selifelse :: sel', Sifthenelse _ s1 s2 => select_stmt s2 sel'
-  | Selloop :: sel', Sloop s => select_stmt s sel'
+  | Selseqleft, Some (Ssequence s1 s2) => Some s1
+  | Selseqright, Some (Ssequence s1 s2) => Some s2
+  | Selifthen, Some (Sifthenelse _ s1 s2) => Some s1
+  | Selifelse, Some (Sifthenelse _ s1 s2) => Some s2
+  | Selloop, Some (Sloop s) => Some s
   | _, _ => None
   end.
-        
+
+Definition select_stmt (stmt: statement) (sel: selector) : option statement :=
+  fold_right select_stmt_aux (Some stmt) sel.
+
+(* (** Maybe we can use fold_right to implement select_stmt and reverse *)
+(* the selectors to simplify the proof *) *)
+(* Fixpoint select_stmt (stmt: statement) (sel: selector) : option statement := *)
+(*   match sel, stmt with *)
+(*   | nil, _ => Some stmt *)
+(*   | Selseqleft :: sel', Ssequence s1 s2 => select_stmt s1 sel' *)
+(*   | Selseqright :: sel', Ssequence s1 s2 => select_stmt s2 sel' *)
+(*   | Selifthen :: sel', Sifthenelse _ s1 s2 => select_stmt s1 sel' *)
+(*   | Selifelse :: sel', Sifthenelse _ s1 s2 => select_stmt s2 sel' *)
+(*   | Selloop :: sel', Sloop s => select_stmt s sel' *)
+(*   | _, _ => None *)
+(*   end. *)
+
+(* Change in place the statement resided in this selector to an another
+statement. And return the modified statement *)
+(** TODO: we do not want to use [rev] *)
+Fixpoint update_stmt_aux (root: statement) (sel: selector) (stmt: statement): option statement :=
+  match sel, root with
+  | nil, _ => Some stmt
+  | Selseqleft :: sel', Ssequence s1 s2 =>
+      match (update_stmt_aux s1 sel' stmt) with
+      | Some s1' => Some (Ssequence s1' s2)
+      | None => None
+      end
+  | Selseqright :: sel', Ssequence s1 s2 =>      
+      match (update_stmt_aux s2 sel' stmt) with
+      | Some s2' => Some (Ssequence s1 s2')
+      | None => None
+      end
+  | Selifthen :: sel', Sifthenelse e s1 s2 =>
+      match (update_stmt_aux s1 sel' stmt) with
+      | Some s1' => Some (Sifthenelse e s1' s2)
+      | None => None
+      end
+  | Selifelse :: sel', Sifthenelse e s1 s2 =>
+      match (update_stmt_aux s2 sel' stmt) with
+      | Some s2' => Some (Sifthenelse e s1 s2')
+      | None => None
+      end
+  | Selloop :: sel', Sloop s =>
+      match (update_stmt_aux s sel' stmt) with
+      | Some s' => Some (Sloop s')
+      | None => None
+      end
+  | _, _ => None
+  end.
+
+Definition update_stmt (root: statement) (sel: selector) (stmt: statement): option statement :=
+  update_stmt_aux root (rev sel) stmt.
+
 
 (** ** Control flow graph based on selector *)
 
@@ -72,38 +125,6 @@ Definition get_stmt (stmt: statement) (cfg: rustcfg) (pc: node) : option stateme
   | None => None
   end.
 
-(* Change in place the statement resided in this selector to an another
-statement. And return the modified statement *)
-Fixpoint update_stmt (root: statement) (sel: selector) (stmt: statement): option statement :=
-  match sel, root with
-  | nil, _ => Some stmt
-  | Selseqleft :: sel', Ssequence s1 s2 =>
-      match (update_stmt s1 sel' stmt) with
-      | Some s1' => Some (Ssequence s1' s2)
-      | None => None
-      end
-  | Selseqright :: sel', Ssequence s1 s2 =>      
-      match (update_stmt s2 sel' stmt) with
-      | Some s2' => Some (Ssequence s1 s2')
-      | None => None
-      end
-  | Selifthen :: sel', Sifthenelse e s1 s2 =>
-      match (update_stmt s1 sel' stmt) with
-      | Some s1' => Some (Sifthenelse e s1' s2)
-      | None => None
-      end
-  | Selifelse :: sel', Sifthenelse e s1 s2 =>
-      match (update_stmt s2 sel' stmt) with
-      | Some s2' => Some (Sifthenelse e s1 s2')
-      | None => None
-      end
-  | Selloop :: sel', Sloop s =>
-      match (update_stmt s sel' stmt) with
-      | Some s' => Some (Sloop s')
-      | None => None
-      end
-  | _, _ => None
-  end.
 
 (** ** Genenrate CFG from a statement *)
 
@@ -323,7 +344,7 @@ Fixpoint transl_stmt (end_node: node) (stmt: statement) (sel: selector) (succ: n
   let transl_stmt := transl_stmt end_node in
   match stmt with
   | Sskip =>
-      add_instr (Isel sel succ)
+      ret succ
   | Sassign p e =>
       add_instr (Isel sel succ)
   | Sassign_variant p enum_id fid e =>
@@ -331,18 +352,18 @@ Fixpoint transl_stmt (end_node: node) (stmt: statement) (sel: selector) (succ: n
   | Sbox p e =>
       add_instr (Isel sel succ)
   | Ssequence stmt1 stmt2 =>
-      do succ2 <- transl_stmt stmt2 (sel ++ [Selseqright]) succ cont brk;
-      do succ1 <- transl_stmt stmt1 (sel ++ [Selseqleft]) succ2 cont brk;
+      do succ2 <- transl_stmt stmt2 (Selseqright :: sel) succ cont brk;
+      do succ1 <- transl_stmt stmt1 (Selseqleft :: sel) succ2 cont brk;
       ret succ1
   | Sifthenelse e stmt1 stmt2 =>
-      do n1 <- transl_stmt stmt1 (sel ++ [Selifthen]) succ cont brk;
-      do n2 <- transl_stmt stmt2 (sel ++ [Selifelse]) succ cont brk;
+      do n1 <- transl_stmt stmt1 (Selifthen :: sel) succ cont brk;
+      do n2 <- transl_stmt stmt2 (Selifelse :: sel) succ cont brk;
       do n3 <- add_instr (Icond e n1 n2);
       ret n3
   | Sloop stmt =>
       do loop_jump_node <- reserve_instr;
       (* The succ in function body is loop_start *)
-      do body_start <- transl_stmt stmt (sel ++ [Selloop]) loop_jump_node (Some loop_jump_node) (Some succ);
+      do body_start <- transl_stmt stmt (Selloop :: sel) loop_jump_node (Some loop_jump_node) (Some succ);
       do _ <- update_instr loop_jump_node (Inop body_start);
       (* return loop_jump_node and return body_start are equivalent *)
       ret loop_jump_node
@@ -388,6 +409,30 @@ Definition generate_cfg (stmt: statement): Errors.res (node * rustcfg) :=
 
 End COMPOSITE_ENV.
 
+(* compute the next selector in the execution (i.e., the starting
+selector of the continuation) *)
+Fixpoint next_sel (sel: selector) : selector :=
+  match sel with
+  | [] => []
+  | Selseqleft :: sel1 => Selseqright :: sel1
+  | Selseqright :: sel1 => next_sel sel1
+  | Selifthen :: sel1 => next_sel sel1
+  | Selifelse :: sel1 => next_sel sel1
+  | Selloop :: sel1 => sel
+  end.
+
+
+Definition cont_sel (s: statement) (sel: selector) : selector :=
+  match s with
+  | Sskip => sel
+  | _ => next_sel sel
+  end.
+
+Lemma cont_sel_nil: forall s,
+    cont_sel s [] = [].
+Proof.
+  intros s; destruct s; auto.
+Qed.
 
 (** * Relations between the generated CFG and the source statement *)
 
@@ -398,68 +443,70 @@ End COMPOSITE_ENV.
   terminates normally, branch to node [cont] if the statement reaches
   Scontinue, branch to break if the statement reaches Sbreak and
   branch to [endn] if the statement returns *)
-Inductive tr_stmt (body: statement) (cfg: rustcfg) : statement -> node -> node -> option node -> option node -> node -> Prop :=
-| tr_Sskip: forall pc cont brk endn,
-    tr_stmt body cfg Sskip pc pc cont brk endn
+Inductive tr_stmt (body: statement) (cfg: rustcfg) : statement -> selector -> node -> node -> option node -> option node -> node -> Prop :=
+| tr_Sskip: forall sel pc cont brk endn,    
+    tr_stmt body cfg Sskip sel pc pc cont brk endn
 | tr_Sassign: forall pc next sel p e cont brk endn
     (SEL: cfg ! pc = Some (Isel sel next))
     (STMT: select_stmt body sel = Some (Sassign p e)),
-    tr_stmt body cfg (Sassign p e) pc next cont brk endn
+    tr_stmt body cfg (Sassign p e) sel pc next cont brk endn
 | tr_Sassign_variant: forall pc next sel p e enum_id fid cont brk endn
     (SEL: cfg ! pc = Some (Isel sel next))
     (STMT: select_stmt body sel = Some (Sassign_variant p enum_id fid e)),
-    tr_stmt body cfg (Sassign_variant p enum_id fid e) pc next cont brk endn
+    tr_stmt body cfg (Sassign_variant p enum_id fid e) sel pc next cont brk endn
 | tr_Sbox: forall pc next sel p e cont brk endn
     (SEL: cfg ! pc = Some (Isel sel next))
     (STMT: select_stmt body sel = Some (Sbox p e)),
-    tr_stmt body cfg (Sbox p e) pc next cont brk endn
+    tr_stmt body cfg (Sbox p e) sel pc next cont brk endn
 | tr_Sstoragelive: forall pc next sel id cont brk endn
     (SEL: cfg ! pc = Some (Isel sel next))
     (STMT: select_stmt body sel = Some (Sstoragelive id)),
-    tr_stmt body cfg (Sstoragelive id) pc next cont brk endn
+    tr_stmt body cfg (Sstoragelive id) sel pc next cont brk endn
 | tr_Sstoragedead: forall pc next sel id cont brk endn
     (SEL: cfg ! pc = Some (Isel sel next))
     (STMT: select_stmt body sel = Some (Sstoragedead id)),
-    tr_stmt body cfg (Sstoragedead id) pc next cont brk endn
+    tr_stmt body cfg (Sstoragedead id) sel pc next cont brk endn
 | tr_Sdrop: forall pc next sel p cont brk endn
     (SEL: cfg ! pc = Some (Isel sel next))
     (STMT: select_stmt body sel = Some (Sdrop p)),
-    tr_stmt body cfg (Sdrop p) pc next cont brk endn
+    tr_stmt body cfg (Sdrop p) sel pc next cont brk endn
 | tr_Scall: forall pc next sel p e args cont brk endn
     (SEL: cfg ! pc = Some (Isel sel next))
     (STMT: select_stmt body sel = Some (Scall p e args)),
-    tr_stmt body cfg (Scall p e args) pc next cont brk endn
-| tr_Ssequence: forall s1 s2 n1 n2 n3 cont brk endn
-    (STMT1: tr_stmt body cfg s1 n1 n2 cont brk endn)
-    (STMT2: tr_stmt body cfg s2 n2 n3 cont brk endn),
-    tr_stmt body cfg (Ssequence s1 s2) n1 n3 cont brk endn
-| tr_Sifthenelse: forall s1 s2 e pc n1 n2 endif cont brk endn
-    (STMT1: tr_stmt body cfg s1 n1 endif cont brk endn)
-    (STMT2: tr_stmt body cfg s2 n2 endif cont brk endn)
+    tr_stmt body cfg (Scall p e args) sel pc next cont brk endn
+| tr_Ssequence: forall s1 s2 n1 n2 n3 cont brk endn sel
+    (STMT1: tr_stmt body cfg s1 (Selseqleft :: sel) n1 n2 cont brk endn)
+    (STMT2: tr_stmt body cfg s2 (Selseqright :: sel) n2 n3 cont brk endn),
+    tr_stmt body cfg (Ssequence s1 s2) sel n1 n3 cont brk endn
+| tr_Sifthenelse: forall s1 s2 e pc n1 n2 endif cont brk endn sel
+    (STMT1: tr_stmt body cfg s1 (Selifthen :: sel) n1 endif cont brk endn)
+    (STMT2: tr_stmt body cfg s2 (Selifelse :: sel) n2 endif cont brk endn)
     (SEL: cfg ! pc = Some (Icond e n1 n2)),
-    tr_stmt body cfg (Sifthenelse e s1 s2) pc endif cont brk endn
-| tr_Sloop: forall s next loop_start loop_jump_node cont brk endn
-    (STMT: tr_stmt body cfg s loop_start loop_jump_node (Some loop_jump_node) (Some next) endn)
+    tr_stmt body cfg (Sifthenelse e s1 s2) sel pc endif cont brk endn
+| tr_Sloop: forall s next loop_start loop_jump_node cont brk endn sel
+    (STMT: tr_stmt body cfg s (Selloop :: sel) loop_start loop_jump_node (Some loop_jump_node) (Some next) endn)
     (SEL: cfg ! loop_jump_node = Some (Inop loop_start)),
     (* next is not specific because loop is impossible to terminate
     normally *)
-    tr_stmt body cfg (Sloop s) loop_jump_node next brk cont endn
+    tr_stmt body cfg (Sloop s) sel loop_jump_node next brk cont endn
 (* backward traversal of CFG. [next] node is used in tr_cont, so it
 should matches the AST *)
-| tr_Sbreak: forall brk cont endn next,
-    tr_stmt body cfg Sbreak brk next cont (Some brk) endn
-| tr_Scontinue: forall brk cont endn next,
-    tr_stmt body cfg Scontinue cont next (Some cont) brk endn
+| tr_Sbreak: forall brk cont endn next sel
+    (STMT: select_stmt body sel = Some Sbreak),
+    tr_stmt body cfg Sbreak sel brk next cont (Some brk) endn
+| tr_Scontinue: forall brk cont endn next sel
+    (STMT: select_stmt body sel = Some Scontinue),
+    tr_stmt body cfg Scontinue sel cont next (Some cont) brk endn
 | tr_Sreturn: forall pc sel endn e cont brk
     (SEL: cfg ! pc = Some (Isel sel endn))
     (STMT: select_stmt body sel = Some (Sreturn e)),
-    tr_stmt body cfg (Sreturn e) pc endn cont brk endn
+    tr_stmt body cfg (Sreturn e) sel pc endn cont brk endn
 .
 
 Inductive tr_fun (f: function) (nret: node) : rustcfg -> Prop :=
 | tr_fun_intro: forall entry cfg
     (CFG: generate_cfg f.(fn_body) = OK (entry, cfg))
-    (STMT: tr_stmt f.(fn_body) cfg f.(fn_body) entry nret None None nret)
+    (STMT: tr_stmt f.(fn_body) cfg f.(fn_body) [] entry nret None None nret)
     (RET: cfg ! nret = Some Iend),
     tr_fun f nret cfg.
 
@@ -468,7 +515,7 @@ Inductive tr_fun (f: function) (nret: node) : rustcfg -> Prop :=
 Lemma transl_stmt_charact: forall body sel stmt nret succ cont brk s s' n R,
     select_stmt body sel = Some stmt ->
     transl_stmt nret stmt sel succ cont brk s = Res n s' R ->
-    tr_stmt body s'.(st_code) stmt n succ cont brk nret.
+    tr_stmt body s'.(st_code) stmt sel n succ cont brk nret.
 Admitted.
 
 
@@ -483,6 +530,3 @@ Proof.
   inv GEN. unfold generate_cfg' in GCFG.
   (** TODO: copy some monadInv from RTLgenspec.v *)
 Admitted.
-
-                              
-                             
